src/Pipit.Exp.Causality.fst
@@ -1,0 +1,159 @@
+module Pipit.Exp.Causality
+
+open Pipit.Exp.Base
+open Pipit.Exp.Subst
+open Pipit.Exp.Bigstep
+
+module C = Pipit.Context
+
+(* Causality: does expression `e` have a dependency on the most-recent value of expression `e'`?
+    *)
+let rec direct_dependency (e e': exp) : bool =
+  if e = e' then true
+  else
+  match e with
+  | XVal _ -> false
+  | XVar x' -> false
+  | XPrim2 _ e1 e2 -> direct_dependency e1 e' || direct_dependency e2 e'
+  | XThen e1 e2 -> direct_dependency e1 e' || direct_dependency e2 e'
+  | XPre _ -> false
+  | XMu e1 -> direct_dependency e1 (lift e' 0)
+
+let rec causal (e: exp): bool =
+  match e with
+  | XVal _ -> true
+  | XVar x' -> true
+  | XPrim2 _ e1 e2 -> causal e1 && causal e2
+  | XThen e1 e2 -> causal e1 && causal e2
+  | XPre e1 -> causal e1
+  | XMu e1 -> causal e1 && not (direct_dependency e1 (XVar 0))
+
+// (* Causality: does expression `e` have a dependency on the most-recent value of variable `x`?
+//    Non-causal expressions cannot be evaluated with the bigstep semantics. *)
+// let rec direct_dependency (e: exp) (x: var) : bool =
+//   match e with
+//   | XVal _ -> false
+//   | XVar x' -> x = x'
+//   | XPrim2 _ e1 e2 -> direct_dependency e1 x || direct_dependency e2 x
+//   | XThen e1 e2 -> direct_dependency e1 x || direct_dependency e2 x
+//   | XPre _ -> false
+//   | XMu e1 -> direct_dependency e1 (x + 1)
+
+let rec lift_inj (e e': exp) (x: var):
+  Lemma (ensures (e = e') == (lift e x = lift e' x)) =
+  match e, e' with
+  | XVal _, XVal _ -> ()
+  | XVar _, XVar _ -> ()
+  | XPrim2 p e1 e2, XPrim2 _ e1' e2' ->
+    lift_inj e1 e1' x; lift_inj e2 e2' x
+  | XPre e1, XPre e1' -> lift_inj e1 e1' x
+  | XThen e1 e2, XThen e1' e2' ->
+    lift_inj e1 e1' x; lift_inj e2 e2' x
+  | XMu e1, XMu e1' -> lift_inj e1 e1' (x + 1)
+  | _, _ -> ()
+
+let rec direct_dependency_lift (e e': exp) (x: var):
+    Lemma (ensures direct_dependency e e' == direct_dependency (lift e x) (lift e' x)) (decreases e) =
+  lift_inj e e' x;
+  match e with
+  | XVal _ -> ()
+  | XVar _ -> ()
+  | XPrim2 p e1 e2 ->
+    direct_dependency_lift e1 e' x;
+    direct_dependency_lift e2 e' x;
+    ()
+  | XPre _ -> ()
+  | XThen e1 e2 ->
+    direct_dependency_lift e1 e' x;
+    direct_dependency_lift e2 e' x;
+    ()
+  | XMu e1 ->
+    direct_dependency_lift e1 (lift e' 0) (x + 1);
+    lift_lift_commute e' x 0;
+    ()
+
+let rec direct_dependency_subst (x: var) (x': var { x' < x })
+  (e: exp { ~ (direct_dependency e (XVar x)) })
+  (p: exp { ~ (direct_dependency p (XVar (x - 1))) }):
+    Lemma (ensures ~ (direct_dependency (subst e x' p) (XVar (x - 1)))) (decreases e) =
+  match e with
+  | XVal _ -> ()
+  | XVar x'' -> ()
+  | XPrim2 prim e1 e2 ->
+    direct_dependency_subst x x' e1 p;
+    direct_dependency_subst x x' e2 p
+  | XPre _ -> ()
+  | XThen e1 e2 ->
+    direct_dependency_subst x x' e1 p;
+    direct_dependency_subst x x' e2 p
+  | XMu e1 ->
+    direct_dependency_lift p (XVar (x - 1)) 0;
+    direct_dependency_subst (x + 1) (x' + 1) e1 (lift p 0)
+
+let rec bigstep_no_dep_no_difference (#outer #inner1 #inner2: nat) (e: exp { ~ (direct_dependency e (XVar inner1)) })
+  (streams1: C.table (outer + 1) inner1)
+  (streams2: C.table (outer + 1) inner2)
+  (row: C.vector value outer) (v v': value)
+  (vs: C.vector value (outer + 1))
+  (hBS: bigstep
+    (C.table_map_append streams1 (C.table_map_append (C.table_of_values (v :: row)) streams2))
+    e
+    vs):
+  Tot (bigstep
+        (C.table_map_append streams1 (C.table_map_append (C.table_of_values (v' :: row)) streams2))
+        e vs) (decreases hBS) =
+  let tv  = C.table_of_values (v :: row) in
+  let tv' = C.table_of_values (v' :: row) in
+  let t2  = C.table_map_append tv streams2 in
+  let t2' = C.table_map_append tv' streams2 in
+  let t  = C.table_map_append streams1 t2 in
+  let t' = C.table_map_append streams1 t2' in
+  match hBS with
+  | BSVal _ v ->
+    C.table_const_const t t' v;
+    BSVal _ v
+  | BSVar _ x ->
+    assert (x <> inner1);
+    if x < inner1
+    then
+    begin
+        C.table_index_append_inner1 streams1 t2 x;
+        C.table_index_append_inner1 streams1 t2' x;
+        BSVar _ x
+    end
+    else
+    begin
+        C.table_index_append_inner2 streams1 t2 x;
+        C.table_index_append_inner2 tv streams2 (x - inner1);
+        C.table_index_append_inner2 streams1 t2' x;
+        C.table_index_append_inner2 tv' streams2 (x - inner1);
+        BSVar _ x
+    end
+  | BSPrim2 _ p e1 e2 vs1 vs2 hBS1 hBS2 ->
+    let hBS1' = bigstep_no_dep_no_difference e1 streams1 streams2 row v v' vs1 hBS1 in
+    let hBS2' = bigstep_no_dep_no_difference e2 streams1 streams2 row v v' vs2 hBS2 in
+    BSPrim2 _ p e1 e2 vs1 vs2 hBS1' hBS2'
+  | BSPre s0 ss e1 vs1 hBS1 ->
+    let s0' = C.table_hd t' in
+    BSPre s0' ss e1 vs1 hBS1
+  | BSThen _ e1 e2 vs1 vs2 hBS1 hBS2 ->
+    let hBS1' = bigstep_no_dep_no_difference e1 streams1 streams2 row v v' vs1 hBS1 in
+    let hBS2' = bigstep_no_dep_no_difference e2 streams1 streams2 row v v' vs2 hBS2 in
+    BSThen _ e1 e2 vs1 vs2 hBS1' hBS2'
+  | BSMu _ e1 vs1 hBS1 ->
+    let e1' = subst e1 0 (XMu e1) in
+    direct_dependency_subst (inner1 + 1) 0 e1 (XMu e1);
+    let hBS1' = bigstep_no_dep_no_difference e1' streams1 streams2 row v v' vs1 hBS1 in
+    BSMu _ e1 vs1 hBS1'
+
+
+let bigstep_recursive_XMu (#outer #inner: nat) (e: exp { causal (XMu e) })
+  (streams: C.table (outer + 1) inner)
+  (vs: C.vector value outer) (v v': value)
+  (hBSmu: bigstep streams (XMu e) (v :: vs)):
+    bigstep (C.table_map_append (C.table_of_values (v' :: vs)) streams) e (v :: vs) =
+    let hBS' = bigstep_substitute_XMu e streams _ hBSmu in
+    C.table_map_append_empty1 (C.table_map_append (C.table_of_values (v :: vs)) streams);
+    C.table_map_append_empty1 (C.table_map_append (C.table_of_values (v' :: vs)) streams);
+    bigstep_no_dep_no_difference e (C.table_empty (outer + 1)) streams vs v v' (v :: vs) hBS'
+
