src/Pipit.System.fst
@@ -1,0 +1,113 @@
+(* Transition systems *)
+module Pipit.System
+
+open Pipit.Exp.Base
+open Pipit.Exp.Bigstep
+open Pipit.Exp.Causality
+
+module C = Pipit.Context
+
+(* Step functions are relations so that we can express non-deterministic systems.
+   The recursive dependency for recursive binders XMu is easier to express as a
+   relation too. The result type is `prop`, rather than a computational boolean,
+   because composing the relations requires existential quantifiers. *)
+type stepfun (input: Type) (state: Type) (result: Type) =
+  (* Values of input variables *)
+  i: input ->
+  (* Starting state, or None for initial *)
+  s: option state ->
+  (* New state *)
+  s': state ->
+  (* Return value *)
+  r: result ->
+  prop
+
+(* A system we get from translating an expression *)
+let xsystem (input: nat) (state: Type) = stepfun (C.vector value input) state value
+
+let rec system_of_exp (e: exp) (vars: nat) (#hwf: squash (wf e vars)):
+    state: Type & xsystem vars state =
+  match e with
+  | XVal v ->
+    (| unit, (fun i s s' r -> r == v) |)
+  | XVar x ->
+    (| unit, (fun i s s' r -> r == C.vector_index i x) |)
+  | XPrim2 p e1 e2 ->
+    let (| st1, t1 |) = system_of_exp e1 vars in
+    let (| st2, t2 |) = system_of_exp e2 vars in
+    (| st1 * st2, (fun i s (s1', s2') r ->
+       let s1, s2 = match s with
+         | None -> None, None
+         | Some (s1, s2) -> Some s1, Some s2
+       in
+       exists (r1 r2: value).
+             t1 i s1 s1' r1 /\
+             t2 i s2 s2' r2 /\
+             r == eval_prim2 p r1 r2)
+    |)
+  | XPre e1 ->
+    let (| st1, t1 |) = system_of_exp e1 vars in
+    (| st1 * value, (fun i s (s1', v') r ->
+      let s1, v = match s with
+        | None -> None, xpre_init
+        | Some (s1, v) -> Some s1, v
+      in
+      t1 i s1 s1' v' /\ r == v) |)
+  | XThen e1 e2 ->
+    let (| st1, t1 |) = system_of_exp e1 vars in
+    let (| st2, t2 |) = system_of_exp e2 vars in
+    (| st2, (fun i s s' r ->
+       match s with
+       | None -> exists s1' r'. t1 i None s1' r /\ t2 i None s' r'
+       | Some _ -> t2 i s s' r)
+    |)
+  | XMu e1 ->
+    let (| st1, t1 |) = system_of_exp e1 (vars + 1) in
+    (| st1, (fun (i: C.vector value vars) s s' r ->
+      t1 (r :: i) s s' r) |)
+  
+let rec step0_ok
+  (#vars: nat)
+  (#state: Type)
+  (e: exp { causal e })
+  (t: xsystem vars state)
+  (#hwf: squash (wf e vars))
+  (#hsys: squash (system_of_exp e vars == (| state, t|)))
+  (row: C.vector value vars)
+  (r r': value)
+  (s': state)
+  (hBS: bigstep (C.table1 (C.Row row)) e (C.vector1 r))
+  (#ht: squash (t row None s' r')):
+   Tot (squash (r == r')) (decreases e) =
+ match e with
+ | XVal _ -> ()
+ | XVar _ -> ()
+ | XPrim2 p e1 e2 ->
+   let BSPrim2 _ _ _ _ [r1] [r2] hBS1 hBS2 = hBS in
+   let (| st1, t1 |) = system_of_exp e1 vars in
+   let (| st2, t2 |) = system_of_exp e2 vars in
+   let (s1', s2') = s' <: (st1 * st2) in
+   eliminate exists (r1' r2': value). t1 row None s1' r1' /\ t2 row None s2' r2' /\ r' == eval_prim2 p r1' r2'
+   returns r == r'
+   with hEx. begin
+     let _ = step0_ok e1 t1 row r1 r1' s1' hBS1 in
+     let _ = step0_ok e2 t2 row r2 r2' s2' hBS2 in
+     ()
+   end
+ | XPre e1 -> ()
+ | XThen e1 e2 ->
+   let BSThen _ _ _ [r1] [r2] hBS1 hBS2 = hBS in
+   let (| st1, t1 |) = system_of_exp e1 vars in
+   let (| st2, t2 |) = system_of_exp e2 vars in
+   eliminate exists (s1': st1) (r2': value). t1 row None s1' r' /\ t2 row None s' r2'
+   returns r == r'
+   with hEx. begin
+     let _ = step0_ok e1 t1 row r1 r' s1' hBS1 in
+     ()
+   end
+ | XMu e1 ->
+   let BSMu _ _ [r] hBS1 = hBS in
+   let (| st1, t1 |) = system_of_exp e1 (vars + 1) in
+   let hBS' = bigstep_recursive_XMu #0 e1 (C.table1 (C.Row row)) [] r r' hBS in
+   let _ = step0_ok e1 t1 (r' :: row) r r' s' hBS' in
+   ()
